theories/Malfunction.v
@@ -1,6 +1,6 @@
 From Coq Require Import ssreflect.
 From Coq Require Import ZArith Floats.
-From MetaCoq Require Import bytestring ReflectEq.
+From MetaCoq.Utils Require Import bytestring ReflectEq.
 Module Int63 := Numbers.Cyclic.Int63.Uint63.
 Notation int := Int63.int.
 
